securedrop-protocol/protocol-minimal/proofs/fstar/extraction/Securedrop_protocol_minimal.Journalist.fst
@@ -3,15 +3,15 @@ module Securedrop_protocol_minimal.Journalist
 open FStar.Mul
 open Core_models
 
-include Securedrop_protocol_minimal.Bundle {impl__from__journalist as impl}
-
-include Securedrop_protocol_minimal.Bundle {impl_1__from__journalist as impl_1}
-
 include Securedrop_protocol_minimal.Bundle {t_Journalist as t_Journalist}
 
 include Securedrop_protocol_minimal.Bundle {t_JournalistPublicView as t_JournalistPublicView}
 
-include Securedrop_protocol_minimal.Bundle {impl_2__new as impl_JournalistPublicView__new}
+include Securedrop_protocol_minimal.Bundle {impl__new as impl_JournalistPublicView__new}
+
+include Securedrop_protocol_minimal.Bundle {impl_1__from__journalist as impl_1}
+
+include Securedrop_protocol_minimal.Bundle {impl_2 as impl_2}
 
 include Securedrop_protocol_minimal.Bundle {impl_3 as impl_3}
 
@@ -19,12 +19,8 @@ include Securedrop_protocol_minimal.Bundle {impl_4 as impl_4}
 
 include Securedrop_protocol_minimal.Bundle {impl_5 as impl_5}
 
-include Securedrop_protocol_minimal.Bundle {impl_6 as impl_6}
+include Securedrop_protocol_minimal.Bundle {f_signed_keybundles__impl_5__extract_public_bundle as f_signed_keybundles__impl_5__extract_public_bundle}
 
-include Securedrop_protocol_minimal.Bundle {impl_7 as impl_7}
+include Securedrop_protocol_minimal.Bundle {impl_6__new as impl_Journalist__new}
 
-include Securedrop_protocol_minimal.Bundle {f_signed_keybundles__impl_7__extract_public_bundle as f_signed_keybundles__impl_7__extract_public_bundle}
-
-include Securedrop_protocol_minimal.Bundle {impl_8__new as impl_Journalist__new}
-
-include Securedrop_protocol_minimal.Bundle {impl_8__public as impl_Journalist__public}
+include Securedrop_protocol_minimal.Bundle {impl_6__public as impl_Journalist__public}
